

# Classical Oscillator Model of Dipole Trapping

Mouhamed Mbengue

October 26 2025

## 1 Static Electric Fields and Matter

**1.1** Recall that a polarizable particle exposed to an electric field will have an induced dipole moment of the form:

$$\mathbf{p} = \alpha \mathbf{E} = q \mathbf{d} \quad (1.1)$$

where  $\alpha$  is the polarizability of the particle. If the electric field is nonuniform, then there will be a force acting on the dipole which will draw it to the region of the stronger electric field.

$$\mathbf{F} = (\mathbf{p} \cdot \nabla) \mathbf{E} \quad (1.2)$$

If we apply eq (4.1) from the appendix

$$\begin{aligned} (\mathbf{E} \cdot \nabla) \mathbf{E} &= \frac{1}{2} \nabla E^2 \\ \mathbf{F} &= \frac{\alpha}{2} \nabla E^2 \end{aligned} \quad (1.3)$$

**1.2** Suppose  $E^2$  had a local maximum at point  $P$  so that there is a sphere of radius  $P + c$  such that:

$$E^2(P) > E^2(P + c) \Rightarrow |E(P)| > |E(P + c)|$$

However, we know that if there's no charge in the sphere, then  $E_{inside} = E_{outside}$ . This contradicts the inequality, so there can't be a local maximum which means that it isn't possible to trap particles in a static field.

## 2 Dipole Potential

**2.1** What about time-varying electric fields? Since we are no longer dealing with electrostatics,  $\nabla \times \mathbf{E} \neq 0$ . This means that the application of eq (4.1) from the appendix gives us:

$$(\mathbf{E} \cdot \nabla)\mathbf{E} = \frac{1}{2}\nabla E^2 + (\mathbf{E} \times \frac{\partial \mathbf{B}}{\partial t})$$

Note that:

$$\frac{\partial}{\partial t}(\mathbf{E} \times \mathbf{B}) = \frac{\partial \mathbf{E}}{\partial t} \times \mathbf{B} + \mathbf{E} \times \frac{\partial \mathbf{B}}{\partial t}$$

Since there is no current density,  $\frac{\partial \mathbf{E}}{\partial t} = \nabla \times \mathbf{B}$  so:

$$\frac{\partial}{\partial t}(\mathbf{E} \times \mathbf{B}) = \nabla \times \mathbf{B} \times \mathbf{B} + \mathbf{E} \times \frac{\partial \mathbf{B}}{\partial t}$$

The first term is 0 which leaves:

$$\frac{\partial}{\partial t}(\mathbf{E} \times \mathbf{B}) = \mathbf{E} \times \frac{\partial \mathbf{B}}{\partial t}$$

Finally, the force on a dipole due to a nonuniform, time varying field is:

$$\mathbf{F} = \alpha \left[ \frac{1}{2} \nabla E^2 + \frac{\partial}{\partial t}(\mathbf{E} \times \mathbf{B}) \right] \quad (2.1)$$

recall that:

$$\mathbf{S} = \frac{1}{\mu_0}(\mathbf{E} \times \mathbf{B})$$

So the force can be rewritten as:

$$\mathbf{F} = \alpha \left[ \frac{1}{2} \nabla E^2 + \mu_0 \frac{\partial \mathbf{S}}{\partial t} \right]$$

**2.2** Electric and magnetic fields oscillate at very rapid speeds, much faster than an atom can react. Therefore a more useful value is the time averaged force which we will define to be the dipole force;

$$\mathbf{F}_{\text{dip}} \equiv \langle \mathbf{F} \rangle$$

$$= \left\langle \frac{\alpha}{2} \nabla |E|^2 \right\rangle + \mu_0 \left\langle \frac{\partial \mathbf{S}}{\partial t} \right\rangle$$

$$= \nabla \left\langle \frac{\alpha}{2} |E|^2 \right\rangle + \mu_0 \frac{\partial}{\partial t} \langle \mathbf{S} \rangle$$

The second term will be zero since the time average of the Poynting vector is a constant, this leaves:

$$\mathbf{F}_{\text{dip}} = \left\langle \frac{\alpha}{2} \nabla |E|^2 \right\rangle$$

$\alpha \in \mathbb{C}$  but the time average must be real, so we average over the real parts of the argument instead:

$$\mathbf{F}_{\text{dip}} = \frac{1}{2} \text{Re}(\alpha) \nabla \langle |E|^2 \rangle$$

$$\langle |E|^2 \rangle = \frac{1}{2} |\tilde{E}_0|^2$$

The square of the magnitude of an electric field is related to its intensity by the expression:

$$I = \frac{1}{2} c \varepsilon_0 |\tilde{E}_0|^2$$

In terms of the intensity, the dipole force is therefore:

$$\mathbf{F}_{\text{dip}} = \frac{1}{2c\varepsilon_0} \text{Re}(\alpha) \nabla I$$

This force is conservative which means that it must be the gradient of some potential. So finally we can express the dipole potential as:

$$U_{\text{dip}} = -\frac{1}{2c\varepsilon_0} \text{Re}(\alpha) I \quad (2.2)$$

### 3 Scattering Rate

**3.1** Recall that power is simply work per unit time:

$$P = \frac{W}{t} = q \frac{\Delta V}{t} = qE \frac{d}{\Delta t} = qEv = E\dot{p}$$

Again we take the time average to get the power absorbed:

$$P_{abs} = \langle \dot{p}E \rangle \quad (3.1)$$

A time dependent electric field is usually of the form:

$$E = \tilde{E}_0 e^{i(kz - \omega t)}$$

This means that:

$$\begin{aligned} p &= \alpha \tilde{E}_0 e^{i(kz - \omega t)} \\ \dot{p} &= -i\omega \alpha \tilde{E}_0 e^{i(kz - \omega t)} = -i\omega \alpha E \end{aligned}$$

If we plug this result into eq (3.1):

$$P_{abs} = \omega \langle i\alpha |E|^2 \rangle$$

This time, since  $\alpha$  is being multiplied by  $i$  we need to average over the complex part to get a real value:

$$\begin{aligned} P_{abs} &= \omega \text{Im}(\alpha) \langle |E|^2 \rangle = \frac{\omega}{2} \text{Im}(\alpha) |\tilde{E}_0|^2 \\ P_{abs} &= \frac{\omega}{c\epsilon_0} \text{Im}(\alpha) I \end{aligned} \quad (3.2)$$

If we view the electric field as a stream of photons, each with energy  $\hbar\omega$ , then the number of photons absorbed and then re emitted by the atom over time defines the scattering rate  $\Gamma_{sc}$

$$\begin{aligned} \Gamma_{sc} &= \frac{P_{abs}}{\hbar\omega} \\ \Gamma_{sc} &= \frac{1}{c\epsilon_0 \hbar} \text{Im}(\alpha) I \end{aligned} \quad (3.3)$$

## 4 Polarizability

**4.1** To determine the polarizability of an atom, we consider the Lorentz model of a classical oscillator. In this model, an electron is considered to be bound to the nucleus by a spring with spring constant  $k = m_e \omega_0^2$  where  $\omega_0$  corresponds to the optical transition frequency. From Newton's second law.

$$F_{net} = F_{driving} - F_{damping} + F_{spring} = m_e \ddot{x}$$

The spring force is simply  $-kx = -\omega_0^2 m_e x$  and the driving force comes from the electric field and is  $F_{driving} = qE$  where  $E(t) = \tilde{E}_0 e^{-i\omega t}$ . We are assuming here that the dipole is small so that there is no significant spatial dependence to the electric field in that region.

**4.2** The damping force comes from the fact that the electron will radiate energy as it accelerates. The power radiated by an accelerating charge is given by Larmor's formula:

$$P = \frac{e^2 a^2}{6\pi\epsilon_0 c^3}$$

The force is therefore:

$$F = \frac{P}{v} = \frac{e^2 a^2}{6\pi\epsilon_0 v c^3} = \Gamma m_e \dot{x}$$

Where:

$$\Gamma = \frac{e^2 a^2}{6\pi\epsilon_0 m_e v^2 c^3}$$

Note that  $\frac{a^2}{v^2} = \omega^2$  so

$$F_{damping} = \Gamma \omega \dot{x}$$

Where:

$$\Gamma_\omega = \frac{e^2 \omega^2}{6\pi\epsilon_0 m_e c^3} \quad (4.1)$$

Is the damping rate of the system.

**4.3** If we plug all of this into Newton's second law we are left with;

$$qE - \Gamma_\omega m_e \dot{x} - \omega_0^2 m_e x = m_e \ddot{x}$$

$$\ddot{x} + \Gamma_\omega \dot{x} + \omega_0^2 x = \frac{q\tilde{E}_0}{m_e} e^{-i\omega t} \quad (4.2)$$

The solution will be of the form:

$$x(t) = x_0 e^{-i\omega t}$$

If we plug this result into the ODE then:

$$-x_0 \omega^2 e^{-i\omega t} - i\omega \Gamma_\omega x_0 e^{-i\omega t} + x_0 \omega_0^2 e^{-i\omega t} = \frac{q\tilde{E}_0}{m_e} e^{-i\omega t}$$

The exponentials will cancel and we're left with:

$$x_0 = \frac{q\tilde{E}_0}{m_e} \frac{1}{-\omega^2 - i\omega \Gamma_\omega + \omega_0^2}$$

Recall from eq (1.1) that:

$$p = qx_0 = \frac{q^2 \tilde{E}_0}{m_e} \frac{1}{-\omega^2 - i\omega \Gamma_\omega + \omega_0^2} = \alpha \tilde{E}_0$$

The polarizability is therefore:

$$\alpha = \frac{q^2}{m_e} \frac{1}{\omega_0^2 - \omega^2 - i\omega\Gamma_\omega} \quad (4.3)$$

From equation (4.2)

$$\frac{e^2}{m_e^2} = \frac{6\pi\epsilon_0 c^3}{\omega^2} \Gamma_\omega$$

To remove the dependence of  $\Gamma_\omega$  on  $\omega$  we introduce the on resonance damping rate  $\Gamma$ , this corresponds to the lifetime of the excited state of the atom which is an actual measurable quantity.

$$\Gamma = \Gamma_{\omega_0} = \frac{\omega_0^2}{\omega^2} \Gamma_\omega$$

Finally we conclude that the atomic polarizability will be:

$$\alpha = 6\pi\epsilon_0 c^3 \frac{\Gamma/\omega_0^2}{\omega_0^2 - \omega^2 - i(\omega^3/\omega_0^2)\Gamma} \quad (4.4)$$

## 5 Putting it all together

**5.1** From equation (4.4) the real part of  $\alpha$  will be:

$$Re(\alpha) = \frac{3\pi\epsilon_0 c^3}{\omega_0^3} \left( \frac{\Gamma}{\omega_0 - \omega} + \frac{\Gamma}{\omega_0 + \omega} \right)$$

While the imaginary part will be:

$$Im(\alpha) = \frac{3\pi\epsilon_0 c^3}{2\omega_0^3} \left( \frac{\omega}{\omega_0} \right)^3 \left( \frac{\Gamma}{\omega_0 - \omega} + \frac{\Gamma}{\omega_0 + \omega} \right)^2$$

If we plug these expressions into equations (2.2) and (3.3) we obtain the following expressions for the dipole potential and scattering rate

$$U_{dip}(\mathbf{r}) = -\frac{3\pi c^3}{2\omega_0^3} \left( \frac{\Gamma}{\omega_0 - \omega} + \frac{\Gamma}{\omega_0 + \omega} \right) I(\mathbf{r})$$

$$\Gamma_{sc}(\mathbf{r}) = \frac{3\pi c^2}{2\hbar\omega_0^3} \left( \frac{\omega}{\omega_0} \right)^3 \left( \frac{\Gamma}{\omega_0 - \omega} + \frac{\Gamma}{\omega_0 + \omega} \right)^2 I(\mathbf{r})$$

In most experiments the laser is tuned close to resonance so that the detuning  $\Delta = \omega - \omega_0$  is small. This means that we can apply the rotating wave approximation so that the second term in both expressions is 0 and  $\omega/\omega_0 \approx 1$ . From this we arrive at the final expressions for the dipole potential and scattering rates in terms of the detuning  $\Delta$  and the field intensity  $I(\mathbf{r})$

$$U_{dip}(\mathbf{r}) = \frac{3\pi c^3}{2\omega_0^3} \frac{\Gamma}{\Delta} I(\mathbf{r}) \tag{5.1}$$

$$\Gamma_{sc}(\mathbf{r}) = \frac{3\pi c^2}{2\hbar\omega_0^3} \left( \frac{\Gamma}{\Delta} \right)^2 I(\mathbf{r}) \tag{5.2}$$

These two equations are related by the expression:

$$\hbar\Gamma_{sc} = \frac{\Gamma}{\Delta} U_{dip} \tag{5.3}$$

## 6 Appendix

### 6.1 Vector Product Rule (4) from Griffiths

$$\nabla(\mathbf{A} \cdot \mathbf{B}) = \mathbf{A} \times (\nabla \times \mathbf{B}) + \mathbf{B} \times (\nabla \times \mathbf{A}) + (\mathbf{A} \cdot \nabla)\mathbf{B} + (\mathbf{B} \cdot \nabla)\mathbf{A} \quad (6.1)$$

**6.2** In general, the time average of two sinusoidal/oscillatory functions with the same frequency and wave number will be (Griffiths 5th edition problem 9.12):

$$\langle fg \rangle = \frac{1}{2} \text{Re}(\tilde{f} \tilde{g}^*)$$

where  $\tilde{f}$  and  $\tilde{g}$  are the amplitudes of  $f$  and  $g$  respectively

## 7 References

Introduction to Electrodynamics 5th Edition Chapters 4, 8 and 9

Optical Dipole Traps for Neutral Atoms

Lorenz Model of a Classical Oscillator